README.txt
@@ -2,27 +2,17 @@ computability in lean
 
 notes:
 
-to register a primrec function, you should:
+/-
+When registering a function as being primrec:
+define:
+c_f : the code of f
+c_f_ev : proof that eval c_f = f
+c_f_ev_pr : proof that eval c_f is prim
 
-namespace Nat.RecursiveIn.Code
-construct it:
-def code_sg := comp (prec zero (((Code.const 1).comp left).comp left)) (pair zero .id) 
-
-show the construction is primitive:
-theorem code_sg_prim : code_prim code_sg := by unfold code_sg; repeat constructor
-
-show the construction has some desired behaviour
-theorem code_sg_prop : eval_prim O code_sg = Nat.sg := by
-  simp [code_sg]
-  simp [eval_prim]
-  funext n
-  induction n with
-  | zero => exact rfl
-  | succ n _ => simp
-end Nat.RecursiveIn.Code
-
-results we want follow:
-theorem Nat.PrimrecIn.sg : Nat.PrimrecIn O Nat.sg := by rw [←code_sg_prop]; apply code_prim_prop code_sg_prim
-theorem Nat.Primrec.sg : Nat.Primrec Nat.sg := by exact PrimrecIn.PrimrecIn_Empty PrimrecIn.sg
+When registering a function on codes (g):
+c_g : the function g from codes to codes
+c_g_ev : proof that eval (c_g asd) has the intended behaviour
+c_g_pr : proof that g itself is primrec
+-/
 
 
